theories/paris/examples/prfprp_adaptive.v
@@ -1,0 +1,49 @@
+From clutch Require Import lib.flip.
+From clutch.paris Require Import paris map list prf prp examples.prf_cpa.
+Set Default Proof Using "Type*".
+
+Section prp_prf.
+
+  Variable Key : nat.
+  Variable val_size : nat.
+  Let Input := val_size.
+  Let Output := val_size.
+
+  (** RandML types of the scheme. *)
+  Definition TKey := TInt.
+  Definition TInput := TInt.
+  Definition TOutput := TInt.
+
+  (** We will prove the PRF/PRP switching lemma.
+      We assume that the adversaries are well-typed. *)
+  Variable adv : val.
+  Definition TAdv := ((TInput → TOutput) → TBool)%ty.
+  Variable adv_typed : (∅ ⊢ₜ adv : TAdv).
+  Definition q_calls := q_calls Input.
+  Definition PRF := PRF val_size val_size.
+  Definition PRP := PRP val_size.
+  (* Definition PRP_PRF : val := λ:"b" "adv",
+         if: "b" then PRP #false "adv" #() else PRF #false "adv" #(). *)
+
+  Local Opaque INR.
+
+  Section proofs.
+    Context `{!parisRGS Σ}.
+
+    Theorem PRP_PRF (Q : nat) ε :
+      (INR (fold_left (Nat.add) (seq 0 Q) 0%nat) / INR (S val_size))%R = ε
+      →
+      ↯ ε ⊢ (REL (PRP #false adv #() #Q) << (PRF #false adv #() #Q) : lrel_bool).
+    Proof with (rel_pures_l ; rel_pures_r).
+    Admitted.
+
+    Theorem PRF_PRP (Q : nat) ε :
+      (INR (fold_left (Nat.add) (seq 0 Q) 0%nat) / INR (S val_size))%R = ε
+      →
+      ↯ ε ⊢ (REL (PRF #false adv #() #Q) << (PRP #false adv #() #Q) : lrel_bool).
+    Proof with (rel_pures_l ; rel_pures_r).
+    Admitted.
+
+  End proofs.
+
+End prp_prf.
