theories/paris/examples/symmetric.v
@@ -1,20 +1,7 @@
 From clutch Require Import lib.flip.
 From clutch.paris Require Import paris map list.
+From clutch.paris Require Export bounded_oracle.
 Set Default Proof Using "Type*".
-
-
-Section bounded_oracle.
-  Local Opaque INR.
-
-  (** Bounded Oracles *)
-  Definition q_calls (MAX : Z) : val :=
-    λ:"Q" "f" "g",
-      let: "counter" := ref #0 in
-      λ:"x", if: (BinOp AndOp (! "counter" < "Q") (BinOp AndOp (#0 ≤ "x") ("x" < #MAX)))
-             then ("counter" <- !"counter" + #1 ;; "f" "x")
-             else "g" "x".
-End bounded_oracle.
-
 
 Section symmetric.
 
